multipleSpecWrites/NonSpecPureStep.v
@@ -5,6 +5,7 @@ Require Import Coq.Sets.Ensembles.
 Require Import sets. 
 Require Import SfLib. 
 Require Import Coq.Program.Equality. 
+Require Import erasure. 
 
 Ltac applyHyp :=
   match goal with
@@ -21,54 +22,6 @@ Proof.
   {destruct s2. inversion H. destruct s1; inversion H2. inversion H. apply IHs1 in H2.
    assumption. } Qed. 
 
-Theorem termErasureDeterminism : forall M T M1 M2,
-                                   eraseTerm M T M1 -> eraseTerm M T M2 -> M1 = M2. 
-Proof.
-  intros. generalize dependent M2. induction H; intros; 
-                                   try(inversion H0; reflexivity);
-  try(clear H; clear H0; match goal with
-                           |H:eraseTerm ?T ?T' ?M |- _ => 
-                    inversion H; clear H; applyHyp; applyHyp; subst; reflexivity
-                         end); 
-  try(clear H; match goal with
-                |H : eraseTerm ?T ?T' ?M |- _ =>
-                 inversion H; clear H; applyHyp; subst; reflexivity
-               end). 
-  {inversion H3; subst. apply IHeraseTerm1 in H8. rewrite H8. 
-   apply uniqueThreadPool with (t' := (Tid(maj,min') tid, s1' ++ [sAct (Tid(maj,min'')tid) M'], s2, M)) in H13. 
-   inversion H13. apply lastElementEq in H5. inversion H5. subst. apply IHeraseTerm2 in H12. 
-   subst. reflexivity. assumption. }
-Qed. 
-
-Theorem erasureDeterminism : forall t t1' t2' T, 
-                               eraseThread t T t1' -> 
-                               eraseThread t T t2' -> t1' = t2'.
-Proof.
-  intros. induction H; inversion H0;
-  try(subst; match goal with
-               |H:eraseTerm ?M ?T ?x, H':eraseTerm ?M ?T ?y |- _ =>
-                eapply termErasureDeterminism in H;[rewrite<-H;reflexivity|auto]
-               |H:[] = [] ++ [?x] |- _ => inversion H       
-               |H:[] = ?x ++ [?y] |- _ => destruct x; inversion H
-               |H:?s1++[?x]=?s2++[?y]|-_ => apply lastElementEq in H; inversion H
-             end);
-  try(subst; eapply termErasureDeterminism in H12;[rewrite <-H12; reflexivity| auto]);
-  reflexivity. Qed. 
-  
-Theorem eraseHeapDeterminism : forall h h1 h2, 
-                                 eraseHeap h h1 -> eraseHeap h h2 ->
-                                 h1 = h2. 
-Proof.
-  intros. generalize dependent h2. induction H; intros. 
-  {inversion H0. subst. apply IHeraseHeap in H6. assumption. }
-  {inversion H0. subst. apply IHeraseHeap in H4. subst. reflexivity. }
-  {inversion H0; subst. apply IHeraseHeap in H10. assumption. }
-  {inversion H0. subst. apply IHeraseHeap in H9. subst. reflexivity. }
-  {inversion H1. subst. apply IHeraseHeap in H8. subst. 
-   eapply termErasureDeterminism in H0. rewrite <-H0. reflexivity. assumption. }
-  {inversion H0. reflexivity. }
-Qed. 
-
 Ltac copy H := 
   match type of H with
       |?X => assert(X) by apply H
@@ -82,39 +35,6 @@ Ltac cleanup := unfold tSingleton in *; unfold tCouple in *; unfold tAdd in *;
            |H : Couple ?T ?y ?z = Singleton ?t ?x |- _ => symmetry in H
          end). 
 
-
-Inductive eraseContext : ctxt -> pool -> pctxt -> Prop :=
-|eraseCtxtHole : forall T, eraseContext holeCtxt T pholeCtxt
-|eraseCtxtBind : forall T N N' E E', eraseTerm N T N' -> eraseContext E T E' ->
-                                     eraseContext (bindCtxt E N) T (pbindCtxt E' N')
-|eraseCtxtSpec : forall T M M' M'' E E' t maj min min' min'' s1 s2,
-                   eraseContext E T E' -> 
-                   thread_lookup T (Tid(maj,min) t) (Tid(maj,min')t, s1 ++ [sAct (Tid(maj,min'')t) M'], s2, M) ->
-                   eraseTerm M' T M'' ->
-                   eraseContext (specReturnCtxt E (threadId (Tid(maj,min)t))) T 
-                                (pbindCtxt E' (plambda (pbind (incBV 1 M'') (plambda (pret (ppair (pbvar 0)(pbvar 1)))))))
-|eraseCtxtHandle : forall T N N' E E',
-                     eraseTerm N T N' -> eraseContext E T E' ->
-                     eraseContext (handleCtxt E N) T (phandleCtxt E' N')
-.
-
-Theorem ctxtErasureDeterminism : forall E T E1 E2, eraseContext E T E1 -> eraseContext E T E2 ->
-                                                   E1 = E2. 
-Proof.
-  intros. generalize dependent E2. induction H; intros. 
-  {inversion H0; subst. reflexivity. }
-  {inversion H1; subst. apply IHeraseContext in H7. subst. eapply termErasureDeterminism in H. 
-   rewrite <- H. reflexivity. assumption. }
-  {inversion H2; subst. apply IHeraseContext in H9. subst. 
-   apply uniqueThreadPool with (t' := (Tid (maj, min'0) t, s0 ++ [sAct (Tid (maj, min''0) t) M'0], s3, M0)) in H0. 
-   inversion H0; subst. apply lastElementEq in H5. inversion H5; subst. 
-   eapply termErasureDeterminism in H11. rewrite <- H11. reflexivity. assumption. assumption. }
-  {inversion H1; subst. apply IHeraseContext in H7. subst. eapply termErasureDeterminism in H. 
-   rewrite <- H. reflexivity. assumption. }
-Qed. 
-
-Hint Constructors eraseContext eraseTerm. 
-
 Ltac invertHyp :=
   match goal with
       |H : exists e : _, ?x |- _ => inversion H; clear H; subst; try invertHyp
@@ -124,32 +44,6 @@ Ltac invertHyp :=
       |H : eraseContext ?E ?T ?E1, H' : eraseContext ?E ?T ?E2 |- _ => 
        eapply ctxtErasureDeterminism in H; try eassumption; subst; try invertHyp
   end. 
-
-Theorem decomposeErase : forall E e T t', 
-                           eraseTerm (fill E e) T t' -> 
-                           exists E' e', eraseContext E T E' /\ eraseTerm e T e' /\ t' = pfill E' e'.
-Proof. 
-  intros. remember (fill E e). generalize dependent E. generalize dependent e. induction H; intros;
-       try solve[destruct E; inversion Heqt; simpl in *; subst; econstructor; econstructor; eauto]; 
-       try solve[destruct E; inversion Heqt; simpl in *; repeat (match goal with
-       |H:forall e0 E, ?e = fill E e0 -> ?X |- _ => 
-        assert(Z:e = fill holeCtxt e) by reflexivity; apply H in Z;
-       invertHyp; clear H
-       |H:eraseContext holeCtxt ?T ?x |- _ => inversion H; subst
-   end); econstructor; econstructor; eauto].
-  {destruct E; inversion Heqt; simpl in *. 
-   {apply IHeraseTerm1 in H2. invertHyp. econstructor. econstructor. eauto. } 
-   {subst. econstructor. econstructor. eauto. }
-  }
-  {destruct E; inversion Heqt; simpl in *. 
-   {apply IHeraseTerm1 in H2. invertHyp. econstructor. econstructor. eauto. }
-   {subst. econstructor. econstructor. eauto. }
-  }
-  {destruct E; inversion Heqt; simpl in *. 
-   {apply IHeraseTerm1 in H4. invertHyp. econstructor. econstructor. eauto. }
-   {subst. econstructor. econstructor. eauto. }
-  }
-Qed. 
 
 Theorem listNeq : forall (T:Type) l (e:T), l = e::l -> False. 
 Proof.
@@ -164,48 +58,53 @@ Proof.
 Qed. 
 
 Theorem NonSpecPureStep : forall h sh pt pt' tid tid' s1 s2 M M' T T',
-                            step h T (tSingleton (tid,s1,s2,M)) h T (tSingleton(tid',s1,s2,M')) ->
+                            step h T (tSingleton (tid,s1,s2,M)) (OK h T (tSingleton(tid',s1,s2,M'))) ->
                             eraseTerm M tEmptySet pt ->
                             eraseTerm M' tEmptySet pt' ->
                             erasePool T T' ->
                             eraseHeap h sh ->
-                            pstep sh T' (pSingleton pt) sh T' (pSingleton pt').
+                            pstep sh T' (pSingleton pt) (pOK sh T' (pSingleton pt')).
 Proof.
-  intros. inversion H; cleanup.
-  {subst. cleanup. copy H1. apply decomposeErase in H1. invertHyp. inversion H1; subst. copy H10. 
-   apply decomposeEq in H10. subst. copy H0. eapply decomposeErase in H0. invertHyp.  
-   inversion H0; subst. apply PBind. inversion H9. invertHyp. apply pdecomposeDecomposed; auto. }
-  {subst. cleanup. copy H1. apply decomposeErase in H1. invertHyp. inversion H1; subst. copy H10. 
-   apply decomposeEq in H10. subst. copy H0. eapply decomposeErase in H0. invertHyp.  
+  intros. inversion H; cleanup; try solve[
+     match goal with
+         |H:?y = ?x::?y |- _ => apply listNeq in H; inversion H
+         |H:?x::?y = ?y |- _ => symmetry in H; apply listNeq in H; inversion H
+     end]. 
+  {subst. cleanup. copy H1. apply decomposeErase in H1. invertHyp. inversion H1; subst. 
+   apply decomposeEq in H8. subst. eapply decomposeErase in H0. invertHyp. inversion H0. 
+   subst. apply PBind. inversion H6. subst. invertHyp. apply pdecomposeDecomposed. auto. }
+  {subst. cleanup. copy H1. apply decomposeErase in H1. invertHyp. inversion H1; subst. copy H8. 
+   apply decomposeEq in H8. subst. copy H0. eapply decomposeErase in H0. invertHyp.  
    inversion H0; subst. inversion H9. invertHyp. econstructor. apply pdecomposeDecomposed; auto. }
-  {subst. cleanup. copy H1. apply decomposeErase in H1. invertHyp. inversion H1; subst. copy H10. 
-   apply decomposeEq in H10. subst. copy H0. eapply decomposeErase in H0. invertHyp.  
-   inversion H0; subst. inversion H9. invertHyp. eapply pHandle.  apply pdecomposeDecomposed; auto. }
-  {subst. cleanup. copy H1. apply decomposeErase in H1. invertHyp. inversion H1; subst. copy H10. 
-   apply decomposeEq in H10. subst. copy H0. eapply decomposeErase in H0. invertHyp.  
+  {subst. cleanup. copy H1. apply decomposeErase in H1. invertHyp. inversion H1; subst. copy H8. 
+   apply decomposeEq in H8. subst. copy H0. eapply decomposeErase in H0. invertHyp.  
+   inversion H0; subst. inversion H8. invertHyp. eapply pHandle.  apply pdecomposeDecomposed; auto. }
+  {subst. cleanup. copy H1. apply decomposeErase in H1. invertHyp. inversion H1; subst. copy H8. 
+   apply decomposeEq in H8. subst. copy H0. eapply decomposeErase in H0. invertHyp.  
    inversion H0; subst. inversion H9. invertHyp. econstructor. apply pdecomposeDecomposed; auto. }
-  { apply eqImpliesSameSet in H10. unfold Same_set in H10. inversion H10. unfold Included in H5. 
-   assert(Ensembles.In thread (Singleton thread (tid', [], s2, M'))(tid', [], s2, M')). 
-   constructor. apply H5 in H6. inversion H6. }
+  {match goal with
+       |H:tEmptySet = Singleton ?T ?x |- _ => apply eqImpliesSameSet in H; unfold Same_set in H;
+                                              unfold Included in H; inversion H as [Imp1 Imp2];
+                                              assert(INHYP:Ensembles.In T (Singleton T x) x) by constructor;
+                                              apply Imp2 in INHYP; inversion INHYP
+   end. }
   {inversion H4. inversion H6. subst. inversion H10. }
-  {eapply Heap.heapUpdateNeq in H9. exfalso. apply H9. eassumption. intros c. inversion c. 
+  {eapply Heap.heapUpdateNeq in H10. exfalso. apply H10. eassumption. intros c. inversion c. 
    apply listNeq in H21. assumption. }
-  { eapply Heap.heapUpdateNeq in H9. exfalso. apply H9. eassumption. intros c. inversion c. }
-  {destruct h; simpl in H11; inversion H11. destruct p. inversion H11. apply listNeq in H16. 
-   inversion H16. }
-  {inversion H4. inversion H7. subst. inversion H10. }
-  {inversion H7. inversion H8. subst. destruct s1'; inversion H17. }
+  { eapply Heap.heapUpdateNeq in H10. exfalso. apply H10. eassumption. intros c. inversion c. }
+  {apply AddEqSingleton in H4. apply AddEqSingleton in H6. inversion H4. inversion H6.
+   rewrite <- H17 in H21. symmetry in H21. apply listNeq in H21. inversion H21. }
+  {inversion H4. apply listNeq in H10. inversion H10. }
+
+  {inversion H8. subst. inversion H7. destruct s1'; inversion H11. }
   {inversion H8. }
-  {eapply disjointUnionEqSingleton in H4. inversion H4; subst. inversion H10. inversion H17. 
-   constructor. unfold not. intros. inversion H7.  inversion H11; subst. 
-   destruct tid0. destruct p. assert(exists p, thread_lookup TRB (Tid (n,n0)l) p). 
-   econstructor. econstructor. eassumption. reflexivity. contradiction. }
+  {eapply disjointUnionEqSingleton in H4. inversion H4; subst. inversion H13. inversion H17. 
+   constructor. unfold not. intros. inversion H16. inversion H18. apply AddEqSingleton in H4.
+   subst x. subst x0. subst t1. destruct tid0. destruct p. 
+   assert(exists x, thread_lookup TRB (Tid (n, n0) l) x). econstructor. econstructor. 
+   eassumption. reflexivity. contradiction. }
   {inversion H8. }
-  {symmetry in H9. apply listNeq in H9. inversion H9. }
-  {symmetry in H10. apply listNeq in H10. inversion H10. }
-  {symmetry in H10. apply listNeq in H10. inversion H10. }
-  {symmetry in H10. apply listNeq in H10. inversion H10. }
-  {inversion H8; inversion H9; subst. inversion H17. }
+  {inversion H10; inversion H11; subst. inversion H17. }
 Qed. 
 
  
