multipleSpecWrites/eraseRollbackIdempotent.v
@@ -1,0 +1,28 @@
+Require Import NonSpec. 
+Require Import Spec.
+Require Import Coq.Sets.Ensembles. 
+Require Import erasure. 
+Require Import AST. 
+
+
+Theorem rollbackIdempotent : forall tid stack H T H' T' H'' T'', 
+                               rollback tid stack H T H' T' -> 
+                               eraseHeap H H'' -> erasePool T T'' ->
+                               eraseHeap H' H'' /\ erasePool T' T''. 
+Proof.
+  intros. generalize dependent H''. generalize dependent T''. induction H0; intros; subst. 
+  {split; auto. }
+  {destruct s1'. 
+   {(*TODO: this case is vacuous*) admit. }
+   {
+
+
+
+
+
+
+
+
+
+
+
